Add Vptr

lang/Lang.v
@@ -1,4 +1,492 @@
+From Coq Require Import
+     Arith.PeanoNat
+     Lists.List
+     Strings.String
+     Morphisms
+     Setoid
+     RelationClasses.
+
+From ExtLib Require Import
+     Data.String
+     Structures.Monad
+     Structures.Traversable
+     Data.List.
+
+From ITree Require Import
+     ITree
+     ITreeFacts
+     Events.MapDefault
+     Events.StateFacts.
+
 From ITree Require Import
      ITree ITreeFacts.
 
 Import ITreeNotations.
+Import Monads.
+Import MonadNotation.
+Local Open Scope monad_scope.
+Local Open Scope string_scope.
+
+
+Definition var : Set := string.
+
+Inductive val: Type :=
+| Vnat (n: nat)
+| Vptr (contents: list val)
+(* | Vundef *)
+(* | Vnodef *)
+.
+
+(** Expressions are made of variables, constant literals, and arithmetic operations. *)
+Inductive expr : Type :=
+| Var (_ : var)
+| Lit (_ : val)
+| Plus  (_ _ : expr)
+| Minus (_ _ : expr)
+| Mult  (_ _ : expr).
+
+(** The statements are straightforward. The [While] statement is the only
+ potentially diverging one. *)
+
+Inductive stmt : Type :=
+| Assign (x : var) (e : expr)    (* x = e *)
+| Seq    (a b : stmt)            (* a ; b *)
+| If     (i : expr) (t e : stmt) (* if (i) then { t } else { e } *)
+| While  (t : expr) (b : stmt)   (* while (t) { b } *)
+| Skip                           (* ; *)
+| Assume
+| Guarantee
+.
+
+(* ========================================================================== *)
+(** ** Notations *)
+
+Module ImpNotations.
+
+  (** A few notations for convenience.  *)
+  Definition Var_coerce: string -> expr := Var.
+  Definition Lit_coerce: nat -> expr := fun n => Lit (Vnat n).
+  Coercion Var_coerce: string >-> expr.
+  Coercion Lit_coerce: nat >-> expr.
+
+  Bind Scope expr_scope with expr.
+
+  Infix "+" := Plus : expr_scope.
+  Infix "-" := Minus : expr_scope.
+  Infix "*" := Mult : expr_scope.
+
+  Bind Scope stmt_scope with stmt.
+
+  (* Notation "x '←' e" := *)
+  (*   (Assign x e) (at level 60, e at level 50): stmt_scope. *)
+
+  (* Notation "a ';;;' b" := *)
+  (*   (Seq a b) *)
+  (*     (at level 100, right associativity, *)
+  (*      format *)
+  (*        "'[v' a  ';;;' '/' '[' b ']' ']'" *)
+  (*     ): stmt_scope. *)
+
+  (* Notation "'IF' i 'THEN' t 'ELSE' e 'FI'" := *)
+  (*   (If i t e) *)
+  (*     (at level 100, *)
+  (*      right associativity, *)
+  (*      format *)
+  (*        "'[v ' 'IF'  i '/' '[' 'THEN'  t  ']' '/' '[' 'ELSE'  e ']' 'FI' ']'"). *)
+
+  (* Notation "'WHILE' t 'DO' b" := *)
+  (*   (While t b) *)
+  (*     (at level 100, *)
+  (*      right associativity, *)
+  (*      format *)
+  (*        "'[v  ' 'WHILE'  t  'DO' '/' '[v' b  ']' ']'"). *)
+
+  Notation "x '#<-' e" :=
+    (Assign x e) (at level 60, e at level 50): stmt_scope.
+
+  Notation "a '#;' b" :=
+    (Seq a b)
+      (at level 100, right associativity,
+       format
+         "'[v' a  '#;' '/' '[' b ']' ']'"
+      ): stmt_scope.
+
+  Notation "'#if' i 'then' t 'else' e 'fi'" :=
+    (If i t e)
+      (at level 100,
+       right associativity,
+       format
+         "'[v ' '#if'  i '/' '[' 'then'  t  ']' '/' '[' 'else'  e ']' 'fi' ']'").
+
+  Notation "'#while' t 'do' b" :=
+    (While t b)
+      (at level 100,
+       right associativity,
+       format
+         "'[v  ' '#while'  t  'do' '/' '[v' b  ']' ']'").
+
+End ImpNotations.
+
+Import ImpNotations.
+
+(* ========================================================================== *)
+(** ** Semantics *)
+
+(** _Imp_ produces effects by manipulating its variables.  To account for this,
+    we define a type of _external interactions_ [ImpState] modeling reads and
+    writes to global variables.
+
+    A read, [GetVar], takes a variable as an argument and expects the
+    environment to answer with a val, hence defining an event of type
+    [ImpState val].
+
+    Similarly, [SetVar] is a write event parameterized by both a variable and a
+    val to be written, and defines an event of type [ImpState unit], no
+    informative answer being expected from the environment.  *)
+Variant ImpState : Type -> Type :=
+| GetVar (x : var) : ImpState val
+| SetVar (x : var) (v : val) : ImpState unit.
+
+Variant Event: Type -> Type :=
+| NB: Event void
+| UB: Event void
+.
+
+Definition triggerUB {E A} `{Event -< E} : itree E A :=
+  vis UB (fun v => match v: void with end)
+.
+Definition triggerNB {E A} `{Event -< E} : itree E A :=
+  vis NB (fun v => match v: void with end)
+.
+
+Section Denote.
+
+  (** We now proceed to denote _Imp_ expressions and statements.
+      We could simply fix in stone the universe of events to be considered,
+      taking as a semantic domain for _Imp_ [itree ImpState X]. That would be
+      sufficient to give meaning to _Imp_, but would prohibit us from relating this
+      meaning to [itree]s stemmed from other entities. Therefore, we
+      parameterize the denotation of _Imp_ by a larger universe of events [eff],
+      of which [ImpState] is assumed to be a subevent. *)
+
+  Context {eff : Type -> Type}.
+  Context {HasImpState : ImpState -< eff}.
+  Context {HasEvent : Event -< eff}.
+
+  (** _Imp_ expressions are denoted as [itree eff val], where the returned
+      val in the tree is the val computed by the expression.
+      In the [Var] case, the [trigger] operator smoothly lifts a single event to
+      an [itree] by performing the corresponding [Vis] event and returning the
+      environment's answer immediately.
+      A constant (literal) is simply returned.
+      Usual monadic notations are used in the other cases: we can [bind]
+      recursive computations in the case of operators as one would expect. *)
+
+  Fixpoint denote_expr (e : expr) : itree eff val :=
+    match e with
+    | Var v     => trigger (GetVar v)
+    | Lit n     => ret n
+    | Plus a b  => l <- denote_expr a ;; r <- denote_expr b ;;
+                     match l, r with
+                     | Vnat l, Vnat r => ret (Vnat (l + r))
+                     | _, _ => triggerUB
+                     end
+    | Minus a b => l <- denote_expr a ;; r <- denote_expr b ;;
+                     match l, r with
+                     | Vnat l, Vnat r => ret (Vnat (l - r))
+                     | _, _ => triggerUB
+                     end
+    | Mult a b  => l <- denote_expr a ;; r <- denote_expr b ;;
+                     match l, r with
+                     | Vnat l, Vnat r => ret (Vnat (l - r))
+                     | _, _ => triggerUB
+                     end
+    end.
+
+  (** We turn to the denotation of statements. As opposed to expressions,
+      statements do not return any val: their semantic domain is therefore
+      [itree eff unit]. The most interesting construct is, naturally, [while].
+
+      To define its meaning, we make use of the [iter] combinator provided by
+      the [itree] library:
+
+      [iter : (A -> itree E (A + B)) -> A -> itree E B].
+
+      The combinator takes as argument the body of the loop, i.e. a function
+      that maps inputs of type [A], the accumulator, to an [itree] computing
+      either a new [A] that can be fed back to the loop, or a return val of
+      type [B]. The combinator builds the fixpoint of the body, hiding away the
+      [A] argument from the return type.
+
+      Compared to the [mrec] and [rec] combinators introduced in
+      [Introduction.v], [iter] is more restricted in that it naturally
+      represents tail recursive functions.  It, however, enjoys a rich equational
+      theory: its addition grants the type of _continuation trees_ (named
+      [ktree]s in the library), a structure of _traced monoidal category_.
+
+      We use [loop] to first build a new combinator [while].
+      The accumulator degenerates to a single [unit] val indicating
+      whether we entered the body of the while loop or not. Since the
+      the operation does not return any val, the return type is also
+      taken to be [unit].
+      That is, the right tag [inr tt] says to exit the loop,
+      while the [inl tt] says to continue. *)
+
+  Definition while (step : itree eff (unit + unit)) : itree eff unit :=
+    iter (C := Kleisli _) (fun _ => step) tt.
+
+  (** Casting vals into [bool]:  [0] corresponds to [false] and any nonzero
+      val corresponds to [true].  *)
+  Definition is_true (v : val) : bool :=
+    match v with
+    | Vnat n => if (n =? 0)%nat then false else true
+    | _ => true (**** YJ: We are assuming type checking here. (reference != null) ****)
+    end
+  .
+
+  (** The meaning of Imp statements is now easy to define.  They are all
+      straightforward, except for [While], which uses our new [while] combinator
+      over the computation that evaluates the conditional, and then the body if
+      the former was true.  *)
+  Fixpoint denote_imp (s : stmt) : itree eff unit :=
+    match s with
+    | Assign x e =>  v <- denote_expr e ;; trigger (SetVar x v)
+    | Seq a b    =>  denote_imp a ;; denote_imp b
+    | If i t e   =>
+      v <- denote_expr i ;;
+      if is_true v then denote_imp t else denote_imp e
+
+    | While t b =>
+      while (v <- denote_expr t ;;
+	           if is_true v
+             then denote_imp b ;; ret (inl tt)
+             else ret (inr tt))
+
+    | Skip => ret tt
+    | Assume => triggerUB
+    | Guarantee => triggerNB
+    end.
+
+End Denote.
+
+(* ========================================================================== *)
+(** ** EXAMPLE: Factorial *)
+
+Section Example_Fact.
+
+  (** We briefly illustrate the language by writing the traditional factorial.
+      example.  *)
+
+  Open Scope expr_scope.
+  Open Scope stmt_scope.
+  Variable input: var.
+  Variable output: var.
+
+  (* Definition fact (n:nat): stmt := *)
+  (*   input ← n;;; *)
+  (*   output ← 1;;; *)
+  (*   WHILE input *)
+  (*   DO output ← output * input;;; *)
+  (*      input  ← input - 1. *)
+  Definition fact (n:nat): stmt :=
+    input #<- n#;
+    output #<- 1#;
+    #while input
+    do output #<- output * input#;
+       input  #<- input - 1.
+
+  (** We have given _a_ notion of denotation to [fact 6] via [denote_imp].
+      However, this is naturally not actually runnable yet, since it contains
+      uninterpreted [ImpState] events.  We therefore now need to _handle_ the
+      events contained in the trees, i.e. give a concrete interpretation of the
+      environment.  *)
+
+End Example_Fact.
+
+(* ========================================================================== *)
+(** ** Interpretation *)
+
+(* begin hide *)
+From ITree Require Import
+     Events.MapDefault.
+
+From ExtLib Require Import
+     Core.RelDec
+     Structures.Maps
+     Data.Map.FMapAList.
+
+(** These enable typeclass instances for Maps keyed by strings and vals *)
+Instance RelDec_string : RelDec (@eq string) :=
+  { rel_dec := fun s1 s2 => if string_dec s1 s2 then true else false}.
+
+Instance RelDec_string_Correct: RelDec_Correct RelDec_string.
+Proof.
+  constructor; intros x y.
+  split.
+  - unfold rel_dec; simpl.
+    destruct (string_dec x y) eqn:EQ; [intros _; apply string_dec_sound; assumption | intros abs; inversion abs].
+  - intros EQ; apply string_dec_sound in EQ; unfold rel_dec; simpl; rewrite EQ; reflexivity.
+Qed.
+(* end hide *)
+
+(** We provide an _ITree event handler_ to interpret away [ImpState] events.  We
+    use an _environment event_ to do so, modeling the environment as a
+    0-initialized map from strings to vals.  Recall from [Introduction.v] that
+    a _handler_ for the events [ImpState] is a function of type [forall R, ImpState R
+    -> M R] for some monad [M].  Here we take for our monad the special case of
+    [M = itree E] for some universe of events [E] required to contain the
+    environment events [mapE] provided by the library. It comes with an event
+    interpreter [interp_map] that yields a computation in the state monad.  *)
+Definition handle_ImpState {E: Type -> Type} `{(mapE var (Vnat 0)) -< E}:
+  ImpState ~> itree E :=
+  fun _ e =>
+    match e with
+    | GetVar x => lookup_def x
+    | SetVar x v => insert x v
+    end.
+
+(** We now concretely implement this environment using ExtLib's finite maps. *)
+Definition env := alist var val.
+
+(** Finally, we can define an evaluator for our statements.
+   To do so, we first denote them, leading to an [itree ImpState unit].
+   We then [interp]ret [ImpState] into [mapE] using [handle_ImpState], leading to
+   an [itree (mapE var val) unit].
+   Finally, [interp_map] interprets the latter [itree] into the state monad,
+   resulting in an [itree] free of any event, but returning the final
+   _Imp_ env.
+ *)
+(* SAZ: would rather write something like the following:
+ h : E ~> M A
+ h' : F[void1] ~> M A
+forall eff, {pf:E -< eff == F[E]} (t : itree eff A)
+        interp pf h h' t : M A
+*)
+
+Definition interp_imp  {E A} (t : itree (ImpState +' E) A) :
+  stateT env (itree E) A :=
+  let t' := interp (bimap handle_ImpState (id_ E)) t in
+  interp_map t'.
+
+Definition handle_Event
+  : Event ~> itree void1 :=
+  fun T e =>
+    match e with
+    | UB => ITree.spin
+    | NB => ITree.spin
+    end
+.
+(* Definition handle_Event {E: Type -> Type}: Event ~> itree void1 := *)
+(*   fun _ e => *)
+(*     match e with *)
+(*     | GetVar x => lookup_def x *)
+(*     | SetVar x v => insert x v *)
+(*     end. *)
+
+Definition interp_Event {E A} (t: itree (Event +' E) A): itree (void1 +' E) A :=
+  let t' := interp (bimap handle_Event (id_ E)) t in
+  t'.
+
+Definition interp_Event2 {A} (t: itree (Event) A): itree (void1) A :=
+  let t' := interp (handle_Event) t in
+  t'.
+
+Variable s: stmt.
+Check (denote_imp s).
+Check interp_imp (denote_imp s) empty.
+Check (@interp_Event _ _ (interp_imp (denote_imp s) empty)).
+Check (interp_Event2 (interp_imp (denote_imp s) empty)).
+
+Definition eval_imp2 (s: stmt) : itree void1 (env * unit)
+  := (interp_Event2 (interp_imp (denote_imp s) empty))
+.
+
+Definition eval_imp (s: stmt) {E} : itree (void1 +' E) (env * unit) :=
+  interp_Event (interp_imp (denote_imp s) empty).
+
+Fail Definition eval_imp (s: stmt) : itree void1 (env * unit) :=
+  interp_imp (denote_imp s) empty.
+
+(** Equipped with this evaluator, we can now compute.
+    Naturally since Coq is total, we cannot do it directly inside of it.
+    We can either rely on extraction, or use some fuel.
+ *)
+Definition test_assume := eval_imp2 Assume.
+                            
+(* Definition test_interp : itree IO unit -> bool := fun t => *)
+Definition stmt_Assume: stmt := Assume.
+Compute (burn 200 (eval_imp2 (fact "input" "output" 6))).
+Compute (burn 200 (eval_imp2 Assume)).
+Compute (burn 200 (eval_imp2 Guarantee)).
+Compute (burn 200 (eval_imp (fact "input" "output" 6))).
+Compute (burn 200 (eval_imp Assume)).
+Compute (burn 200 (eval_imp Guarantee)).
+Goal forall E R, (burn 200 (@ITree.spin E R)) = (burn 2 (ITree.spin)).
+  reflexivity.
+Qed.
+
+Goal forall E, (burn 200 (@eval_imp Assume E)) = (burn 2 (eval_imp Assume)).
+  reflexivity.
+Qed.
+
+Require Extraction.
+
+Extraction "impK.ml" stmt_Assume.
+Extraction "impK.ml" eval_imp.
+Definition main := (burn 100 (eval_imp2 stmt_Assume)).
+Extraction "impK.ml" main.
+(* Extraction "impK.ml" burn. *)
+
+(* ========================================================================== *)
+Section InterpImpProperties.
+  (** We can lift the underlying equational theory on [itree]s to include new
+      equations for working with [interp_imp].
+
+      In particular, we have:
+         - [interp_imp] respects [≈]
+         - [interp_imp] commutes with [bind].
+
+      We could justify more equations than just the ones below.  For instance,
+      _Imp_ programs also respect a coarser notation of equivalence for the
+      [env] state.  We exploit this possibility to implement optimzations
+      at the _Asm_ level (see AsmOptimizations.v).
+   *)
+
+  Context {E': Type -> Type}.
+  Notation E := (ImpState +' E').
+
+  (** This interpreter is compatible with the equivalence-up-to-tau. *)
+  Global Instance eutt_interp_imp {R}:
+    Proper (@eutt E R R eq ==> eq ==> @eutt E' (prod (env) R) (prod _ R) eq)
+           interp_imp.
+  Proof.
+    repeat intro.
+    unfold interp_imp.
+    unfold interp_map.
+    rewrite H0. eapply eutt_interp_state_eq; auto.
+    rewrite H. reflexivity.
+  Qed.
+
+  (** [interp_imp] commutes with [bind]. *)
+  Lemma interp_imp_bind: forall {R S} (t: itree E R) (k: R -> itree E S) (g : env),
+      (interp_imp (ITree.bind t k) g)
+    ≅ (ITree.bind (interp_imp t g) (fun '(g',  x) => interp_imp (k x) g')).
+  Proof.
+    intros.
+    unfold interp_imp.
+    unfold interp_map.
+    repeat rewrite interp_bind.
+    repeat rewrite interp_state_bind.
+    apply eqit_bind. red. intros.
+    destruct a as [g'  x].
+    simpl.
+    reflexivity.
+    reflexivity.
+  Qed.
+
+End InterpImpProperties.
+
+
+
+(** We now turn to our target language, in file [Asm].v *)
+
