hfc/Mpool.v
@@ -1,0 +1,57 @@
+From Coq Require Import
+     Arith.PeanoNat
+     Lists.List
+     Strings.String
+     Morphisms
+     Setoid
+     RelationClasses.
+
+From ExtLib Require Import
+     Data.String
+     Structures.Monad
+     Structures.Traversable
+     Data.List.
+
+From ITree Require Import
+     ITree
+     ITreeFacts
+     Events.MapDefault
+     Events.StateFacts.
+
+From ITree Require Import
+     ITree ITreeFacts.
+
+Import ITreeNotations.
+Import Monads.
+Import MonadNotation.
+Local Open Scope monad_scope.
+Local Open Scope string_scope.
+
+
+
+From HafniumCore
+     Require Import Lang.
+Import ImpNotations.
+
+Set Implicit Arguments.
+
+
+
+
+Module MPOOL.
+
+  (*
+     ONLY: fallback & chunk_list
+   *)
+
+  Definition entry_size: nat := 4096.
+
+  Definition init: stmt :=
+    "p" #<- "entry_size"
+  .
+
+  Definition fini: stmt :=
+  .
+
+End MPOOL.
+
